tuned and refactored Network_Security_Policy_Verification

thys/Network_Security_Policy_Verification/Lib/ML_GraphViz.thy
@@ -14,6 +14,7 @@ signature GRAPHVIZ =
 sig
   val open_viewer: bool Unsynchronized.ref
 
+  (*function to modify the printing of a node name*)
   val default_tune_node_format: term -> string -> string
 
   (* edges is a term of type ('a \<times> 'a) list *)
@@ -21,9 +22,15 @@ sig
   (* @{context} default_tune_node_format (edges_format \<times> edges)list*)
   val visualize_graph: Proof.context -> (term -> string -> string) -> term -> int
 
-  (* @{context} default_tune_node_format (edges_format \<times> edges)list*)
-  val visualize_graph_pretty: Proof.context -> (term -> string -> string) -> (string * term) list-> int
+  (* @{context} default_tune_node_format (edges_format \<times> edges)list graphviz_header*)
+  val visualize_graph_pretty: Proof.context -> (term -> string -> string) -> (string * term) list -> string-> int
 
+  (* helper function.
+     @{context} tune_node_format node *)
+  val node_to_string: Proof.context -> (term -> string -> string) ->  term -> string
+  val term_to_string: Proof.context ->  term -> string;
+  val term_to_string_safe: Proof.context ->  term -> string;
+  val term_to_string_html: Proof.context ->  term -> string;
 end
 
 structure Graphviz: GRAPHVIZ =
@@ -32,7 +39,7 @@ struct
 (*if set to false, graphviz will not be run and not pdf will be opened. Include ML_GraphViz_Disable.thy to run in batch mode.*)
 val open_viewer = Unsynchronized.ref true
 
-val default_tune_node_format = (fn _ => I)
+val default_tune_node_format: term -> string -> string = (fn _ => I)
 
 fun write_to_tmpfile (t: string): Path.T = 
   let 
@@ -42,10 +49,52 @@ fun write_to_tmpfile (t: string): Path.T =
     writeln ("using tmpfile " ^ p_str); File.write p (t^"\n"); p
   end
 
-fun evaluate_term ctxt edges = 
+fun evaluate_term (ctxt: Proof.context) edges = 
   case Code_Evaluation.dynamic_value ctxt edges of
     SOME x => x
-  | NONE => error "ML_GraphViz: failed to evaluate edges"
+  | NONE => error "ML_GraphViz: failed to evaluate term"
+
+
+fun is_valid_char c =
+  (c <= #"z" andalso c >= #"a") orelse (c <= #"Z" andalso c >= #"A") orelse
+  (c <= #"9" andalso c >= #"0")
+
+val sanitize_string =
+  String.map (fn c => if is_valid_char c then c else #"_")
+
+
+fun term_to_string (ctxt: Proof.context) (t: term) : string = 
+  (*n |> Syntax.pretty_term ctxt |> Pretty.string_of |> ATP_Util.unyxml*)
+  let
+    val ctxt' = Config.put show_markup false ctxt;
+  in Print_Mode.setmp [] (Syntax.string_of_term ctxt') t
+  end;
+
+
+fun term_to_string_safe ctxt (n: term) : string = 
+  let
+    val str = term_to_string ctxt n
+  in
+    if sanitize_string str <> str then (warning ("String  "^str^" contains invalid characters!"); sanitize_string str)
+     else str end;
+
+local
+  val sanitize_string_html =
+    String.map (fn c => if (is_valid_char c orelse c = #" " orelse (c <= #"/" andalso c >= #"(")
+                            orelse c = #"|" orelse c = #"=" orelse c = #"?" orelse c = #"!" orelse c = #"_"
+                            orelse c = #"[" orelse c = #"}") then c else #"_")
+in
+  fun term_to_string_html ctxt (n: term) : string = 
+    let
+      val str = term_to_string ctxt n
+    in
+      if sanitize_string_html str <> str then (warning ("String  "^str^" contains invalid characters!"); sanitize_string_html str)
+       else str end
+end;
+
+fun node_to_string ctxt (tune_node_format: term -> string -> string) (n: term) : string = 
+  n |> term_to_string ctxt |> tune_node_format n
+  handle Subscript => error ("Subscript Exception in node_to_string for string "^( Pretty.string_of (Syntax.pretty_term ctxt n)));
 
 local
 
@@ -75,34 +124,30 @@ local
         (*some pdf viewers do not like it if we delete the pdf file they are currently displaying*)
       end
 
-  fun is_valid_char c =
-    (c <= #"z" andalso c >= #"a") orelse (c <= #"Z" andalso c >= #"A") orelse
-    (c <= #"9" andalso c >= #"0")
-
-  val sanitize_string =
-    String.map (fn c => if is_valid_char c then c else #"_")
-
   fun format_dot_edges ctxt tune_node_format trm =
     let
-      fun format_node t = t |> Syntax.pretty_term ctxt |> Pretty.string_of |> YXML.content_of |> tune_node_format t |> sanitize_string
+      fun format_node t = let val str = node_to_string ctxt tune_node_format t in
+                              if sanitize_string str <> str then
+                                (warning ("Node "^str^" contains invalid characters!"); sanitize_string str)
+                              else str
+                            end;
       fun format_dot_edge (t1, t2) = format_node t1 ^ " -> " ^ format_node t2 ^ ";\n"
     in
-      writeln "TODO: name clashes?"; map format_dot_edge trm
+      map format_dot_edge trm
     end
 
-  fun apply_dot_header es =
-    "digraph graphname {\n" ^ implode es ^ "}"
+  fun apply_dot_header header edges =
+    "digraph graphname {\n#header\n" ^ header ^"\n#edges\n\n"^ implode edges ^ "}"
 in
-  fun visualize_graph_pretty ctxt tune_node_format Es : int =
+  fun visualize_graph_pretty ctxt tune_node_format Es (header:string): int =
     let 
       val evaluated_edges = map (fn (str, t) => (str, evaluate_term ctxt t)) Es
-      val edge_to_string =
-        HOLogic.dest_list #> map HOLogic.dest_prod #> format_dot_edges ctxt tune_node_format #> implode
+      val edge_to_string = HOLogic.dest_list #> map HOLogic.dest_prod #> format_dot_edges ctxt tune_node_format #> implode
       val formatted_edges = map (fn (str, t) => str ^ "\n" ^ edge_to_string t) evaluated_edges
     in
       if !open_viewer then (* only run the shell commands if not disabled by open_viewer *)
         (
-          apply_dot_header formatted_edges
+          apply_dot_header header formatted_edges
           |> write_to_tmpfile
           |> paint_graph Graphviz_Platform_Config.executable_pdf_viewer Graphviz_Platform_Config.executable_dot
         )
@@ -112,7 +157,7 @@ in
   end
 
 fun visualize_graph ctxt tune_node_format edges =
-  visualize_graph_pretty ctxt tune_node_format [("", edges)]
+  visualize_graph_pretty ctxt tune_node_format [("", edges)] "#TODO add header here"
 
 end;
 *}
