thys/Network_Security_Policy_Verification/Examples/Distributed_WebApp.thy
@@ -1,0 +1,254 @@
+theory Distributed_WebApp
+imports "../TopoS_Impl"
+begin
+
+(*Isabelle 2013-2*)
+
+
+section{*Distributed Web Application Example*}
+
+text{* 
+    The symbolic policy names are of type @{typ vString}. This is just a wrapped string, e.g. @{term "V ''WebFrnt''"}
+*}
+abbreviation "V\<equiv>TopoS_Vertices.V"
+
+text{*We start with the empty policy, only the entities are defined.*}
+definition policy :: "vString list_graph" where
+    "policy \<equiv> \<lparr> nodesL = [V ''WebFrnt'', V ''DB'', V ''Log'', V ''WebApp'', V ''INET''],
+                edgesL = [] \<rparr>"
+
+text{*Sanity check*}
+lemma "valid_list_graph policy" by eval
+(*proof by eval means we have executable code to show the lemma.*)
+
+
+text{*Defining the security invariants*}
+definition LogSink_m::"(vString SecurityInvariant)" where
+  "LogSink_m \<equiv> new_configured_list_SecurityInvariant SINVAR_LIB_Sink \<lparr> 
+          node_properties = [V ''Log'' \<mapsto> Sink], 
+          model_global_properties = () 
+          \<rparr>"
+
+text{*
+0 - unclassified
+1 - confidential
+*}
+--"trusted: can access any security clearance, privacy-level 0: can reveal to anyone. I.e. can declassify"
+definition BLP_m::"(vString SecurityInvariant)" where
+    "BLP_m \<equiv> new_configured_list_SecurityInvariant SINVAR_LIB_BLPtrusted \<lparr> 
+          node_properties = [V ''DB'' \<mapsto> \<lparr> privacy_level = 1, trusted = False \<rparr>,
+                             V ''Log'' \<mapsto> \<lparr> privacy_level = 1, trusted = False \<rparr>,
+                             V ''WebApp'' \<mapsto> \<lparr> privacy_level = 0, trusted = True \<rparr> 
+                             ], 
+          model_global_properties = () 
+          \<rparr>"
+
+definition Subnet_m::"(vString SecurityInvariant)" where
+    "Subnet_m \<equiv> new_configured_list_SecurityInvariant SINVAR_LIB_SubnetsInGW \<lparr> 
+          node_properties = [V ''DB'' \<mapsto> Member,
+                             V ''Log'' \<mapsto> Member,
+                             V ''WebApp'' \<mapsto> Member,
+                             V ''WebFrnt'' \<mapsto> InboundGateway (*DMZ*)
+                             ], 
+          model_global_properties = () 
+          \<rparr>"
+
+
+definition DBACL_m::"(vString SecurityInvariant)" where
+    "DBACL_m \<equiv> new_configured_list_SecurityInvariant SINVAR_LIB_CommunicationPartners \<lparr> 
+          node_properties = [V ''DB'' \<mapsto> Master [V ''WebApp''],
+                             V ''WebApp'' \<mapsto> Care
+                             ], 
+          model_global_properties = () 
+          \<rparr>"
+
+text{*The list of security invariants*}
+definition "security_invariants = [Subnet_m, BLP_m, LogSink_m, DBACL_m]"
+
+text{*All security invariants are fulfilled (obviously, the policy permits no flows).*}
+lemma "all_security_requirements_fulfilled security_invariants policy" by eval
+
+text{*Obviously, no policy rules violate the security invariants.*}
+lemma "implc_get_offending_flows security_invariants policy = []" by eval
+
+
+text{*We generate the maximum security policy.*}
+definition "max_policy = generate_valid_topology security_invariants \<lparr>nodesL = nodesL policy, edgesL = List.product (nodesL policy) (nodesL policy) \<rparr>"
+
+
+text{*Calculating the maximum policy (executing it).*}
+value "max_policy"
+lemma "max_policy = 
+   \<lparr>nodesL = [V ''WebFrnt'', V ''DB'', V ''Log'', V ''WebApp'', V ''INET''],
+    edgesL = [(V ''WebFrnt'', V ''WebFrnt''), (V ''WebFrnt'', V ''Log''), (V ''WebFrnt'', V ''WebApp''), (V ''WebFrnt'', V ''INET''), (V ''DB'', V ''DB''),
+              (V ''DB'', V ''Log''), (V ''DB'', V ''WebApp''), (V ''Log'', V ''Log''), (V ''WebApp'', V ''WebFrnt''), (V ''WebApp'', V ''DB''),
+              (V ''WebApp'', V ''Log''), (V ''WebApp'', V ''WebApp''), (V ''WebApp'', V ''INET''), (V ''INET'', V ''WebFrnt''), (V ''INET'', V ''INET'')]\<rparr>"
+by eval (*proof by eval means it can be directly executed*)
+
+text{*
+Visualizing the maximum policy
+*}
+ML{*
+visualize_graph @{context} @{term "security_invariants"} @{term "max_policy"};
+*}
+
+text{*The maximum policy also fulfills all security invariants. *}
+lemma "all_security_requirements_fulfilled security_invariants max_policy" by eval
+text{*This holds in general: @{thm generate_valid_topology_sound}.*}
+
+text{*fine-tuning generated policy.*}
+definition "my_policy = \<lparr>nodesL = [V ''WebFrnt'', V ''DB'', V ''Log'', V ''WebApp'', V ''INET''],
+    edgesL = [(V ''WebFrnt'', V ''WebFrnt''), (V ''WebFrnt'', V ''Log''), (V ''WebFrnt'', V ''WebApp''), (V ''DB'', V ''DB''), (V ''DB'', V ''Log''),
+              (V ''DB'', V ''WebApp''), (V ''Log'', V ''Log''), (V ''WebApp'', V ''WebFrnt''), (V ''WebApp'', V ''DB''), (V ''WebApp'', V ''Log''), (V ''WebApp'', V ''WebApp''),
+              (V ''WebApp'', V ''INET''), (V ''INET'', V ''WebFrnt''), (V ''INET'', V ''INET'')]\<rparr>"
+lemma "all_security_requirements_fulfilled security_invariants my_policy" by eval
+lemma "set (edgesL my_policy) \<subset> set (edgesL max_policy)" by eval
+
+text{*
+The diff to the maximum policy.
+*}
+ML_val{*
+visualize_edges @{context} @{term "edgesL my_policy"} 
+    [("edge [dir=\"arrow\", style=dashed, color=\"#3399FF\", constraint=false]", @{term "[e \<leftarrow> edgesL max_policy. e \<notin> set (edgesL my_policy)]"})] ""; 
+*}
+
+
+
+section{*A stateful implementation*}
+definition "stateful_policy = generate_valid_stateful_policy_IFSACS my_policy security_invariants"
+value "stateful_policy"
+
+text{*the stateful compliance criteria*}
+
+text{*No information flow violations*}
+  lemma "all_security_requirements_fulfilled (get_IFS security_invariants) (stateful_list_policy_to_list_graph stateful_policy)" by eval
+  
+  text{*No access control side effects*}
+  lemma "\<forall> F \<in> set (implc_get_offending_flows (get_ACS security_invariants) (stateful_list_policy_to_list_graph stateful_policy)).
+            set F \<subseteq> set (backlinks (flows_stateL stateful_policy)) - (set (flows_fixL stateful_policy))" by eval
+
+  text{*In general, the calculated stateful policy complies with the security policy: @{thm generate_valid_stateful_policy_IFSACS_stateful_policy_compliance}*}
+
+text{*Visualizing the stateful policy.*}
+ML_val{*
+visualize_edges @{context} @{term "flows_fixL stateful_policy"} 
+    [("edge [dir=\"arrow\", style=dashed, color=\"#FF8822\", constraint=false]", @{term "flows_stateL stateful_policy"})] ""; 
+*}
+
+
+subsection{*Exporting to Network Security Mechanism Configurations*}
+
+
+text{*Space-separated policy dump*}
+ML_val{*
+iterate_edges_ML @{context} @{term "flows_fixL stateful_policy"}
+  (fn (v1,v2) => writeln (""^v1^" "^v2) )
+  (fn _ => () )
+  (fn _ => () );
+
+writeln "# stateful answers";
+iterate_edges_ML @{context} @{term "flows_stateL stateful_policy"}
+  (fn (v1,v2) => writeln (v2^" "^v1) )
+  (fn _ => () )
+  (fn _ => () )
+*}
+
+text{*firewall -- classical use case*}
+ML_val{*
+
+(*header*)
+writeln ("echo 1 > /proc/sys/net/ipv4/ip_forward"^"\n"^
+         "# flush all rules"^"\n"^
+         "iptables -F"^"\n"^
+         "#default policy for FORWARD chain:"^"\n"^
+         "iptables -P FORWARD DROP");
+
+iterate_edges_ML @{context}  @{term "flows_fixL stateful_policy"}
+  (fn (v1,v2) => writeln ("iptables -A FORWARD -i $"^v1^"_iface -s $"^v1^"_ipv4 -o "^v2^"_iface -d $"^v2^"_ipv4 -j ACCEPT"^" # "^v1^" -> "^v2) )
+  (fn _ => () )
+  (fn _ => () );
+
+iterate_edges_ML @{context} @{term "flows_stateL stateful_policy"}
+  (fn (v1,v2) => writeln ("iptables -I FORWARD -m state --state ESTABLISHED -i $"^v2^"_iface -s $"^v2^"_ipv4 -o $"^v1^"_iface -d $"^v1^"_ipv4 # "^v2^" -> "^v1^" (answer)") )
+  (fn _ => () )
+  (fn _ => () )
+*}
+
+text{*firewall -- OpenVPN scenario*}
+ML_val{*
+
+(*header*)
+writeln ("echo 1 > /proc/sys/net/ipv4/ip_forward"^"\n"^
+         "# flush all rules"^"\n"^
+         "iptables -F"^"\n"^
+         "#default policy for FORWARD chain:"^"\n"^
+         "iptables -P FORWARD DROP");
+
+fun iface (s: string): string =
+  if s = "INET" then "eth0" else "tun0";
+
+iterate_edges_ML @{context} @{term "[(s,r) \<leftarrow> flows_fixL stateful_policy. s \<noteq> r]"}
+  (fn (v1,v2) => writeln ("iptables -A FORWARD -i "^iface v1^" -s $"^v1^"_ipv4 -o "^iface v2^" -d $"^v2^"_ipv4 -j ACCEPT") )
+  (fn _ => () )
+  (fn _ => () );
+
+iterate_edges_ML @{context} @{term "flows_stateL stateful_policy"}
+  (fn (v1,v2) => writeln ("iptables -I FORWARD -m state --state ESTABLISHED -i "^iface v2^" -s $"^v2^"_ipv4 -o "^iface v1^" -d $"^v1^"_ipv4 -j ACCEPT") )
+  (fn _ => () )
+  (fn _ => () )
+*}
+
+
+lemma "set (flows_stateL stateful_policy) \<subseteq> set (flows_fixL stateful_policy)" by eval
+
+definition stateful_flows :: "(vString \<times> vString) list" where
+  "stateful_flows \<equiv> [(src, dst) \<leftarrow> flows_stateL stateful_policy. src \<noteq> dst]"
+value "stateful_flows"
+
+definition stateless_flows :: "(vString \<times> vString) list" where
+  "stateless_flows \<equiv> [(src, dst) \<leftarrow> flows_fixL stateful_policy. src \<noteq> dst \<and> (src, dst) \<notin> set stateful_flows]"
+value "stateless_flows"
+
+text{*OpenFlow Flow table Rules*}
+ML_val{*
+fun ARP (src: string) (dst: string): string =
+  "# ARP Request\n"^
+	"in_port=${port_"^src^"} dl_src=${mac_"^src^"} dl_dst=ff:ff:ff:ff:ff:ff arp arp_sha=${mac_"^src^"} "^
+	"arp_spa=${ip4_"^src^"} arp_tpa=${ip4_"^dst^"} priority=40000 action=mod_dl_dst:${mac_"^dst^"},output:${port_"^dst^"}"^"\n"^
+	"# ARP Reply\n"^
+	"dl_src=${mac_"^dst^"} dl_dst=${mac_"^src^"} arp arp_sha=${mac_"^dst^"} "^
+	"arp_spa=${ip4_"^dst^"} arp_tpa=${ip4_"^src^"} priority=40000 action=output:${port_"^src^"}";
+
+local
+  fun IPv4_helper (priority: int) (nw_src_wildcard: bool) (nw_dst_wildcard: bool) (src: string) (dst: string): string =
+    let
+      val nw_src = (if nw_src_wildcard then "*" else "${ip4_"^src^"}");
+      val nw_dst = (if nw_dst_wildcard then "*" else "${ip4_"^dst^"}");
+    in
+      "in_port=${port_"^src^"} dl_src=${mac_"^src^"} ip nw_src="^nw_src^" "^
+      "nw_dst="^nw_dst^" priority="^(Int.toString priority)^" action=mod_dl_dst:${mac_"^dst^"},output:${port_"^dst^"}"
+    end;
+in
+  fun IPv4 (src: string) (dst: string): string =
+    if dst = "INET" then
+      IPv4_helper 30000 false true src dst
+    else if src = "INET" then
+      IPv4_helper 30000 true false src dst
+    else
+      IPv4_helper 40000 false false src dst
+      ;
+end;
+
+iterate_edges_ML @{context} @{term "stateful_flows"}
+  (fn (v1,v2) => writeln ((ARP v1 v2) ^ "\n" ^ (ARP v2 v1) ^ "\n" ^ (IPv4 v1 v2) ^ "\n" ^ (IPv4 v2 v1) ^"\n"))
+  (fn _ => () )
+  (fn _ => () );
+
+iterate_edges_ML @{context} @{term "stateless_flows"}
+  (fn (v1,v2) =>  writeln ((ARP v1 v2) ^ "\n" ^ (IPv4 v1 v2) ^ "\n"))
+  (fn _ => () )
+  (fn _ => () )
+*}
+
+
+end
